\documentclass{beamer}
\usepackage{listings}
\lstset{
%language=C,
frame=single, 
breaklines=true,
columns=fullflexible
}
\usepackage{subcaption}
\usepackage{url}
\usepackage{tikz}
\usepackage{tkz-euclide} % loads  TikZ and tkz-base
%\usetkzobj{all}
\usetikzlibrary{calc,math}
\usepackage{float}
\newcommand\norm[1]{\left\lVert#1\right\rVert}
\renewcommand{\vec}[1]{\mathbf{#1}}
\usepackage[export]{adjustbox}
\usepackage[utf8]{inputenc}
\usepackage{amsmath}
\usepackage{multicol}
\usetheme{Boadilla}
\providecommand{\pr}[1]{\ensuremath{\Pr\left(#1\right)}}

\title{(GATE 2001 (MA), Q. 2.24)}
\author{Vaibhav Chhabra - AI20BTECH11022}
\date{}
\begin{document}

\begin{frame}
\titlepage
\end{frame}
\begin{frame}
\frametitle{Question}
\begin{block}{}
Let $(X,Y)$ be a two-dimensional random variable such that $E(X)=E(Y)=3$, $Var(X)=Var(Y)=1$ and $Cov(X,Y)=1/2$.
Then, $P(|X-Y|>6)$ is
\begin{enumerate}
\begin{multicols}{2}
    \item less than 1/6
    \item equal to 1/2
    \item equal to 1/3
    \item greater than 1/2
\end{multicols}
\end{enumerate}
\end{block}
\end{frame}

\begin{frame}
\frametitle{Solution}
Given,
\begin{align} \label{eq-1}
    E(X)=E(Y)=3
\end{align}
\begin{align}
    Var(X)=Var(Y)=1
\end{align}
\begin{align}
    Cov(X,Y)=1/2
\end{align}
Now,
\begin{align}
    Var(X)=E(X^2)-(E(X))^2
\end{align}
Substituting given values, we get,
\begin{align}
    1=E(X^2)-3^2
\end{align}
So,
\begin{align} \label{eq-2}
    E(X^2)=10
\end{align}
Similarly for $Y$,
\begin{align} \label{eq-3}
    E(Y^2)=10
\end{align}
\end{frame}
\begin{frame}
\frametitle{Solution}
Also,
\begin{align}
    Cov(X,Y)=E(XY)-E(X)E(Y)
\end{align}
Substituting given values, we get,
\begin{align}
    1/2=E(XY)-(3)(3)
\end{align}
So,
\begin{align} \label{eq-4}
    E(XY)=19/2
\end{align}
Let $Z$ be a random variable defined as
\begin{align} \label{eq-5}
    Z=X-Y
\end{align}
Then using \eqref{eq-1},
\begin{align} \label{eq-6}
    E(Z)=E(X-Y)=E(X)-E(Y)=0
\end{align}
\end{frame}

\begin{frame}
\frametitle{Solution}
Now, using \eqref{eq-6}
\begin{align}
    Var(Z)=E(Z^2)-(E(Z))^2=E(Z^2)
\end{align}
\begin{align}
    Var(Z)=E((X-Y)^2)
\end{align}
\begin{align}
    Var(Z)=E(X^2)+E(Y^2)-2E(XY)
\end{align}
Using \eqref{eq-2}, \eqref{eq-3} and \eqref{eq-4},
\begin{align}
    Var(Z)=10+10-2 \times 19/2
\end{align}
\begin{align} \label{eq-7}
    Var(Z)=1
\end{align}
\end{frame}
\begin{frame}
\frametitle{Chebychev's Inequality}
\begin{theorem}
(Chebychev's Inequality)\ Let T be an arbitrary random variable, with finite mean E(T), then for all $a>0$,
\begin{align}
    \pr{|T-E(T)| \geq a} \leq \dfrac{Var(T)}{a^2}
\end{align}
\end{theorem}

Proof: \\
Let T be a random variable with probablility distribution function $f(T)$ and $a>0$ be any real number.
Then,
\begin{align}
    \pr{|T-E(T)| \geq a}= \int_{-\infty}^{-E(T)-a}f(T)dT +  \int_{E(T)+a}^{\infty}f(T)dT
\end{align}
\begin{align} \label{eq-8}
    \pr{|T-E(T)| \geq a}= \int_{|T-E(T)| \geq a}f(T)dT
\end{align}
\end{frame}
\begin{frame}
\frametitle{}
Now,
\begin{align}
    Var(T)= \int_{-\infty}^{\infty}(T-E(T))^2f(T)dT \nonumber \\ \geq \int_{|T-E(T)|\geq a}(T-E(T))^2f(T)dT \nonumber \\ \geq a^2\int_{|T-E(T)|\geq a}f(T)dT
\end{align}
So, we finally get,
\begin{align}
    Var(T) \geq a^2\int_{|T-E(T)|\geq a}f(T)dT
\end{align}
Using \eqref{eq-8},
\begin{align}
    Var(T) \geq a^2\pr{|T-E(T)| \geq a}
\end{align}
Or,
\begin{align}
    \pr{|T-E(T)| \geq a} \leq \dfrac{Var(T)}{a^2}
\end{align}
\end{frame}

\begin{frame}
\frametitle{Solution Contd.}
Applying Chebychev's Inequality for $Z$ with $a=6$, we get,
\begin{align}
    \pr{|Z-E(Z)| \geq 6} \leq \dfrac{Var(Z)}{6^2}
\end{align}
Using \eqref{eq-6} and \eqref{eq-7},
\begin{align}
    \pr{|Z-0| \geq 6} \leq \dfrac{1}{36}
\end{align}
As $Z=X-Y$,
\begin{align}
    \pr{|X-Y| \geq 6} \leq \dfrac{1}{36}
\end{align}
So, option 1 is correct.
\end{frame}

\end{document}